theories/L6_PCPS/Heap/closure_conversion_correct.v
@@ -18,21 +18,57 @@ Module ClosureConversionCorrect (H : Heap).
 
   Module Size := Size H.
   
-  Import H Size.Compat.LR.Sem.Equiv Size.Compat.LR.Sem.Equiv.Defs Size.Compat.LR.Sem Size.Compat.LR
-         Size.Compat Size.
+  Import H Size.Compat.LR.Sem.Equiv Size.Compat.LR.Sem.Equiv.Defs Size.Compat.LR.Sem
+         Size.Compat.LR Size.Compat Size.
   
   Variable clo_tag : cTag.
+
+  Inductive Forall2_P {A B : Type} (P : A -> Prop)
+            (R : A -> B -> Prop) : list A -> list B -> Prop :=
+    Forall2_nil : Forall2_P P R [] []
+  | Forall2_cons_P :
+      forall (x : A) (y : B) (l : list A) (l' : list B),
+        (~ P x ->  R x y) -> 
+        Forall2_P P R l l' ->
+        Forall2_P P R (x :: l) (y :: l').
+
+  Lemma Forall2_P_monotonic_strong {A B} (P : A -> Prop)
+        (R R' : A -> B -> Prop) l1 l2 :
+    (forall x1 x2,
+       List.In x1 l1 ->
+       List.In x2 l2 -> ~ P x1 -> R' x1 x2 -> R x1 x2) -> 
+    Forall2_P P R' l1 l2 ->
+    Forall2_P P R l1 l2.
+  Proof with (now eauto with Ensembles_DB). 
+    intros Hyp Hf. induction Hf; try now constructor.
+    - constructor; eauto. intros. eapply Hyp; eauto. now constructor.
+      now constructor. eapply IHHf.
+      intros. eapply Hyp. now constructor 2.
+      now constructor 2. eassumption. eassumption.
+  Qed.
+
+  Lemma Forall2_P_monotonic {A B} (P P' : A -> Prop) (R : A -> B -> Prop) l1 l2 :
+    Forall2_P P' R l1 l2 ->
+    P' \subset P -> 
+    Forall2_P P R l1 l2.
+  Proof.
+    intros Hall Hs. induction Hall; eauto.
+    - constructor.
+    - constructor 2; eauto.
+      firstorder.
+  Qed.
   
   (** Invariant about the free variables *) 
   Definition FV_inv (k j : nat) (IP : GIInv) (P : GInv) (b : Inj)
              (rho1 : env) (H1 : heap block) (rho2 : env) (H2 : heap block)
-             (c : cTag) (Γ : var) (FVs : list var) : Prop :=
-    exists (v : value) (vs : list value) (l : loc),
+             (c : cTag) (Scope Funs : Ensemble var) (Γ : var) (FVs : list var) : Prop :=
+    exists (vs : list value) (l : loc),
       M.get Γ rho2 = Some (Loc l) /\
       get l H2 = Some (Constr c vs) /\
-      Forall2 (fun x v' => 
-                 exists v, M.get x rho1 = Some v /\
-                      Res (v, H1) ≺ ^ ( k ; j ; IP ; P ; b) Res (v', H2)) FVs vs.
+      Forall2_P (Scope :|: Funs)
+                (fun (x : var) (v2 : value)  =>
+                   exists v1, M.get x rho1 = Some v1 /\
+                         Res (v1, H1) ≺ ^ ( k ; j ; IP ; P ; b) Res (v2, H2)) FVs vs.
   
   (** Invariant about the functions in the current function definition *)
   Definition Fun_inv (k j : nat) (IP : GIInv) (P : GInv) (b : Inj)
@@ -40,152 +76,390 @@ Module ClosureConversionCorrect (H : Heap).
              (Scope Funs : Ensemble var) (σ : var -> var)  : Prop :=
     (* (exists f, f \in Funs) /\ *)
     forall (f : var),
-     In var Funs f ->
-      exists lf1 lf2,
-        M.get f rho1 = Some lf1 /\ 
-        M.get (σ f) rho2 = Some lf2 /\
-        Res (lf1, H1) ≺ ^ ( k ; j ; IP ; P ; b) Res (lf2, H2).
+    ~ f \in Scope ->
+    f \in Funs ->
+    exists lf1 lf2,
+      M.get f rho1 = Some lf1 /\ 
+      M.get (σ f) rho2 = Some lf2 /\
+      Res (lf1, H1) ≺ ^ ( k ; j ; IP ; P ; b) Res (lf2, H2).
   
   (** Versions without the logical relation. Useful when we're only interested in other invariants. *)
   
   (** Invariant about the free variables *) 
   Definition FV_inv_weak (rho1 : env) (rho2 : env) (H2 : heap block)
-             (c : cTag) (Γ : var) (FVs : list var) : Prop :=
-    exists (v : value) (vs : list value) (l : loc),
+             (c : cTag) (Scope Funs : Ensemble var) (Γ : var) (FVs : list var) : Prop :=
+    exists (vs : list value) (l : loc),
       M.get Γ rho2 = Some (Loc l) /\
       get l H2 = Some (Constr c vs) /\
-      Forall2 (fun x v' => exists v, M.get x rho1 = Some v) FVs vs.
+      Forall2_P (Scope :|: Funs)
+                (fun (x : var) (v2 : value)  =>
+                   exists v1, M.get x rho1 = Some v1) FVs vs.
   
   (** Invariant about the functions in the current function definition *)
   Definition Fun_inv_weak (rho1 : env) (H1 : heap block) (rho2 : env) (H2 : heap block)
              (Scope Funs : Ensemble var) (σ : var -> var) : Prop :=
     (* (exists f, f \in Funs \\ Scope) /\ *)
     forall (f : var),
-      In var Funs f ->
+      ~ f \in Scope ->
+      f \in Funs  ->    
       exists lf1 lf2,
         M.get f rho1 = Some lf1 /\ 
         M.get (σ f) rho2 = Some lf2.
   
-  (** * Lemmas about [V_inv] *)
+  (** * Lemmas about [FV_inv] *)
 
+  Require Import Logic.ClassicalFacts.
+
+  Axiom excluded_middle : excluded_middle. 
+  
   Lemma FV_inv_image_post (k j : nat) (GII : GIInv) (GI : GInv) (b : Inj)
              (rho1 : env) (H1 : heap block) (rho2 : env) (H2 : heap block)
-             (c : cTag) (Γ : var) (FVs : list var) :
-    FV_inv k j GII GI b rho1 H1 rho2 H2 c Γ FVs ->    
-    image b ((post H1 ^ j) (env_locs rho1 (FromList FVs))) <-->
+             (c : cTag) (Scope Funs : Ensemble var) (Γ : var) (FVs : list var) :
+    FV_inv k j GII GI b rho1 H1 rho2 H2 c Scope Funs Γ FVs ->    
+    image b ((post H1 ^ j) (env_locs rho1 (FromList FVs \\ (Scope :|: Funs)))) \subset
     (post H2 ^ j) (post H2 (env_locs rho2 ([set Γ]))).
-  Proof.
-    intros Hfv. destruct Hfv as (v & vs & l & Hget1 & Hget2 & Hall).
-    rewrite (proper_post_n H2); [| now rewrite env_locs_Singleton; eauto; apply post_Singleton; eauto ].
-    simpl. clear Hget1 Hget2. induction Hall.
-    - simpl. rewrite post_n_Empty_set.
-      eapply Same_set_trans; [| eapply image_Empty_set with (g := b) ].
-      rewrite proper_post_n; [| rewrite FromList_nil, env_locs_Empty_set; reflexivity ].
-      rewrite post_n_Empty_set. reflexivity.
-    - rewrite proper_post_n; [| rewrite FromList_cons, env_locs_Union; reflexivity ].
-      simpl. rewrite !post_n_Union, image_Union.
-      eapply Same_set_Union_compat; [| now eauto ].
-      destruct H as [v' [Hget' Hres]].
-      rewrite proper_post_n; [| now eapply env_locs_Singleton; eauto ].
+  Proof with (now eauto with Ensembles_DB).
+    intros (vs & l & Hget1 & Hget2 & Hall).
+    eapply Included_trans; [| eapply post_n_set_monotonic;
+                              rewrite env_locs_Singleton; eauto; simpl;
+                              rewrite post_Singleton; eauto; reflexivity ].
+    clear Hget1 Hget2.
+    induction Hall.
+    - eapply Included_trans.
+      eapply image_monotonic. eapply post_n_set_monotonic.
+      rewrite FromList_nil. rewrite Setminus_Empty_set_abs_r.
+      rewrite env_locs_Empty_set. reflexivity.
+      rewrite post_n_Empty_set, image_Empty_set...
+    - rewrite proper_post_n;
+      [| rewrite FromList_cons, Setminus_Union_distr, env_locs_Union
+         ; try reflexivity ]. 
+      destruct (excluded_middle ((Scope :|: Funs) x)).
+      + rewrite proper_post_n;
+        [| rewrite Setminus_Included_Empty_set, env_locs_Empty_set,
+           Union_Empty_set_neut_l; try reflexivity ].
+        eapply Included_trans. eassumption.
+        eapply post_n_set_monotonic. simpl...
+        eapply Singleton_Included. eassumption.
+      +rewrite proper_post_n;
+        [| rewrite Setminus_Disjoint; try reflexivity ].
+       simpl. rewrite !post_n_Union, image_Union.
+       eapply Included_Union_compat; eauto.
+       destruct (H H0) as [v1 [Hget1 Hres]].
+       rewrite proper_post_n; 
+        [| rewrite env_locs_Singleton; eauto; reflexivity ].
       eapply cc_approx_val_image_eq. eassumption.
+      eapply Disjoint_Singleton_l; eauto.
   Qed.
 
+  Lemma FV_inv_image_post_eq (k j : nat) (GII : GIInv) (GI : GInv) (b : Inj)
+             (rho1 : env) (H1 : heap block) (rho2 : env) (H2 : heap block)
+             (c : cTag) (Scope Funs : Ensemble var) (Γ : var) (FVs : list var) :
+    FV_inv k j GII GI b rho1 H1 rho2 H2 c Scope Funs Γ FVs ->
+    Disjoint _ (FromList FVs) (Scope :|: Funs) ->
+    image b ((post H1 ^ j) (env_locs rho1 (FromList FVs))) <-->
+    (post H2 ^ j) (post H2 (env_locs rho2 ([set Γ]))).
+  Proof with (now eauto with Ensembles_DB).
+    intros Hfv Hd. split.
+    - eapply Included_trans.
+      eapply image_monotonic. eapply post_n_set_monotonic.
+      rewrite <- (Setminus_Disjoint (FromList FVs)); try eassumption.
+      reflexivity. eapply FV_inv_image_post. eassumption.
+    - destruct Hfv as (vs & l & Hget1 & Hget2 & Hall).
+      eapply Included_trans; [ eapply post_n_set_monotonic;
+                               rewrite env_locs_Singleton; eauto; simpl;
+                               rewrite post_Singleton; eauto; reflexivity |].
+      clear Hget1 Hget2.
+      induction Hall.
+      * simpl. rewrite post_n_Empty_set...
+      * assert (Hneq : ~ (Scope :|: Funs) x).
+        { intros Hc. eapply Hd. constructor; eauto. constructor; eauto. }
+        destruct (H Hneq) as [v1 [Hget1 Hres]].
+        eapply Included_trans;
+        [| eapply image_monotonic; eapply post_n_set_monotonic;
+           rewrite FromList_cons, env_locs_Union, env_locs_Singleton; eauto; reflexivity ]. 
+        simpl. rewrite !post_n_Union, image_Union. 
+        eapply Included_Union_compat; eauto.
+        eapply cc_approx_val_image_eq. eassumption.
+        eapply IHHall.  eapply Disjoint_Included_l; [| eassumption ].
+        rewrite FromList_cons...
+  Qed.
+  
   Lemma FV_inv_j_monotonic (k j' j : nat) (GII : GIInv) (GI : GInv) (b : Inj)
         (rho1 : env) (H1 : heap block) (rho2 : env) (H2 : heap block)
-        (c : cTag) (Γ : var) (FVs : list var) :
-    FV_inv k j GII GI b rho1 H1 rho2 H2 c Γ FVs ->
+        (c : cTag) (Scope Funs : Ensemble var) (Γ : var) (FVs : list var) :
+    FV_inv k j GII GI b rho1 H1 rho2 H2 c Scope Funs Γ FVs ->
     j' <= j ->
-    FV_inv k j' GII GI b rho1 H1 rho2 H2 c Γ FVs.
+    FV_inv k j' GII GI b rho1 H1 rho2 H2 c Scope Funs Γ FVs.
   Proof.
     intros Hfv Hlt. 
-    destruct Hfv as (v & vs & l & Hget1 & Hget2 & Hall).
+    destruct Hfv as (v & vs & Hget1 & Hget2 & Hall).
     repeat eexists; eauto.
-    eapply Forall2_monotonic; [| eassumption ].
-    intros x1 x2 [v' [Hget Hres]]. eexists; split; eauto.
+    eapply Forall2_P_monotonic_strong; [| eassumption ].
+    intros x1 x2 Hin1 Hin3 Hnp [v' [Hget Hres]]; eauto.
+    eexists; split; eauto.
     eapply cc_approx_val_j_monotonic; eauto.
   Qed.
 
+  Lemma FV_inv_monotonic (k k' j : nat) (GII : GIInv) (GI : GInv) (b : Inj)
+        (rho1 : env) (H1 : heap block) (rho2 : env) (H2 : heap block)
+        (c : cTag) (Scope Funs : Ensemble var) (Γ : var) (FVs : list var) :
+    FV_inv k j GII GI b rho1 H1 rho2 H2 c Scope Funs Γ FVs ->
+    k' <= k ->
+    FV_inv k' j GII GI b rho1 H1 rho2 H2 c Scope Funs Γ FVs.
+  Proof.
+    intros Hfv Hlt. 
+    destruct Hfv as (v & vs & Hget1 & Hget2 & Hall).
+    repeat eexists; eauto.
+    eapply Forall2_P_monotonic_strong; [| eassumption ].
+    intros x1 x2 Hin1 Hin3 Hnp [v' [Hget Hres]]; eauto.
+    eexists; split; eauto.
+    eapply cc_approx_val_monotonic; eauto.
+  Qed.
     
   Lemma FV_inv_image_reach_n (k j : nat) (GII : GIInv) (GI : GInv) (b : Inj)
              (rho1 : env) (H1 : heap block) (rho2 : env) (H2 : heap block)
-             (c : cTag) (Γ : var) (FVs : list var) :
-    FV_inv k j GII GI b rho1 H1 rho2 H2 c Γ FVs ->    
-    image b (reach_n H1 j (env_locs rho1 (FromList FVs))) <-->
+             (c : cTag) (Scope Funs : Ensemble var) (Γ : var) (FVs : list var) :
+    FV_inv k j GII GI b rho1 H1 rho2 H2 c Scope Funs Γ FVs ->    
+    image b (reach_n H1 j (env_locs rho1 (FromList FVs \\ (Scope :|: Funs)))) \subset
     (reach_n H2 j (post H2 (env_locs rho2 ([set Γ])))).
   Proof.
-    intros Hfv. split.
-    - intros l' [l [[m [Hm Hr]] Hin]].
-      eapply FV_inv_j_monotonic in Hfv; eauto.
-      eexists m. split; eauto. eapply FV_inv_image_post. eassumption.
-      eexists; split; eauto.
-    - intros l' [m [Hm Hr]].
-      eapply FV_inv_j_monotonic in Hfv; eauto.
-      eapply FV_inv_image_post in Hr; eauto.
-      destruct Hr as [l [Heql Hin]]. eexists; split; eauto.
-      eexists; split; eauto.
+    intros Hfv. 
+    intros l' [l [[m [Hm Hr]] Hin]].
+    eapply FV_inv_j_monotonic in Hfv; eauto.
+    eexists m. split; eauto. eapply FV_inv_image_post. eassumption.
+    eexists; split; eauto.
+
   Qed.
 
   Lemma FV_inv_image_reach (k : nat) (GII : GIInv) (GI : GInv) (b : Inj)
              (rho1 : env) (H1 : heap block) (rho2 : env) (H2 : heap block)
-             (c : cTag) (Γ : var) (FVs : list var) :
-    (forall j, FV_inv k j GII GI b rho1 H1 rho2 H2 c Γ FVs) ->    
+             (c : cTag) (Scope Funs : Ensemble var) (Γ : var) (FVs : list var) :
+    (forall j, FV_inv k j GII GI b rho1 H1 rho2 H2 c Scope Funs Γ FVs) ->    
+    image b (reach' H1 (env_locs rho1 (FromList FVs \\ (Scope :|: Funs)))) \subset
+    (reach' H2 (post H2 (env_locs rho2 ([set Γ])))).
+  Proof.
+    intros Hfv.
+    intros l' [l [[m [Hm Hr]] Heq]].
+    eexists m. split; eauto. eapply FV_inv_image_post. eauto.
+    eexists; split; eauto.
+  Qed.
+
+  Lemma FV_inv_image_reach_n_eq (k j : nat) (GII : GIInv) (GI : GInv) (b : Inj)
+             (rho1 : env) (H1 : heap block) (rho2 : env) (H2 : heap block)
+             (c : cTag) (Scope Funs : Ensemble var) (Γ : var) (FVs : list var) :
+    FV_inv k j GII GI b rho1 H1 rho2 H2 c Scope Funs Γ FVs ->
+    Disjoint _ (FromList FVs) (Scope :|: Funs) ->
+    image b (reach_n H1 j (env_locs rho1 (FromList FVs))) <-->
+    reach_n H2 j (post H2 (env_locs rho2 ([set Γ]))).
+  Proof.
+    intros Hfv. split.
+    - intros l' [l [[m [Hm Hr]] Hin]].
+      eapply FV_inv_j_monotonic in Hfv; eauto.
+      eexists m. split; eauto. eapply FV_inv_image_post_eq. eassumption.
+      eassumption. eexists; split; eauto.
+    - intros l' [m [Hm Hr]].
+      eapply FV_inv_j_monotonic in Hfv; eauto.
+      eapply FV_inv_image_post_eq in Hr; eauto.
+      destruct Hr as [l [Heql Hin]]. eexists; split; eauto.
+      eexists; split; eauto.
+  Qed.
+
+  Lemma FV_inv_image_reach_eq (k : nat) (GII : GIInv) (GI : GInv) (b : Inj)
+             (rho1 : env) (H1 : heap block) (rho2 : env) (H2 : heap block)
+             (c : cTag) (Scope Funs : Ensemble var) (Γ : var) (FVs : list var) :
+    (forall j, FV_inv k j GII GI b rho1 H1 rho2 H2 c Scope Funs Γ FVs) ->
+    Disjoint _ (FromList FVs) (Scope :|: Funs) ->
     image b (reach' H1 (env_locs rho1 (FromList FVs))) <-->
     (reach' H2 (post H2 (env_locs rho2 ([set Γ])))).
   Proof.
     intros Hfv. split.
     - intros l' [l [[m [Hm Hr]] Heq]].
-      eexists m. split; eauto. eapply FV_inv_image_post. eauto.
+      eexists m. split; eauto. eapply FV_inv_image_post_eq; eauto.
       eexists; split; eauto.
     - intros l' [m [Hm Hr]].
-      eapply FV_inv_image_post in Hr; eauto.
+      eapply FV_inv_image_post_eq in Hr; eauto.
       destruct Hr as [l [Heql Hin]]. eexists; split; eauto.
       eexists; split; eauto.
   Qed.
-
-  (** * Lemmas about [FV_inv] *)
-  Lemma FV_inv_weak_in_FV_inv k j P1 P2 rho1 H1 rho2 H2 β c Γ FVs :
-    FV_inv k j P1 P2 β rho1 H1 rho2 H2 c Γ FVs ->
-    FV_inv_weak rho1 rho2 H2 c Γ FVs.
+  
+  Lemma FV_inv_weak_in_FV_inv k j P1 P2 rho1 H1 rho2 H2 β c Scope Funs Γ FVs :
+    FV_inv k j P1 P2 β rho1 H1 rho2 H2 c Scope Funs Γ FVs ->
+    FV_inv_weak rho1 rho2 H2 c Scope Funs Γ FVs.
   Proof.
-    intros (x1 & x2 & l & Hget1 & Hget2 & Hall).
+    intros (x1 & x2  & Hget1 & Hget2 & Hall).
     repeat eexists; eauto.
-    eapply Forall2_monotonic; [| eassumption ].
+    eapply Forall2_P_monotonic_strong; [| eassumption ].
     now firstorder.
   Qed.
 
-  (** * Lemmas about [Fun_inv] *)
+  Lemma FV_inv_set_not_in_FVs_l (k j : nat) (GII : GIInv) (GI : GInv) (b : Inj)
+        (rho1 : env) (H1 : heap block) (rho2 : env) (H2 : heap block)
+        (c : cTag) (Scope Funs : Ensemble var) (Γ : var) (FVs : list var) x v  :
+    FV_inv k j GII GI b rho1 H1 rho2 H2 c Scope Funs Γ FVs ->
+    ~ x \in (FromList FVs \\ (Scope :|: Funs)) ->
+    FV_inv k j GII GI b (M.set x v rho1) H1 rho2 H2 c Scope Funs Γ FVs.
+  Proof.
+    intros (x1 & x2 & Hget1 & Hget2 & Hall).
+    repeat eexists; eauto.
+    eapply Forall2_P_monotonic_strong; [| eassumption ].
+    intros y1 v2 Hin Hnin Hp [v1 [Hget Hall1]].
+    eexists; split; eauto.
+    rewrite M.gso; eauto.
+    intros Hc; subst. eapply H; constructor; eauto. 
+  Qed.
 
+  Lemma FV_inv_set_not_in_FVs_r (k j : nat) (GII : GIInv) (GI : GInv) (b : Inj)
+        (rho1 : env) (H1 : heap block) (rho2 : env) (H2 : heap block)
+        (c : cTag) (Scope Funs : Ensemble var) (Γ : var) (FVs : list var) x v  :
+    FV_inv k j GII GI b rho1 H1 rho2 H2 c Scope Funs Γ FVs ->
+    x <> Γ ->
+    FV_inv k j GII GI b rho1 H1 (M.set x v rho2) H2 c Scope Funs Γ FVs.
+  Proof.
+    intros (x1 & x2 & Hget1 & Hget2 & Hall).
+    repeat eexists; eauto.
+    rewrite M.gso; eauto.
+  Qed. 
+  
+  Lemma FV_inv_set_not_in_FVs (k j : nat) (GII : GIInv) (GI : GInv) (b : Inj)
+        (rho1 : env) (H1 : heap block) (rho2 : env) (H2 : heap block)
+        (c : cTag) (Scope Funs : Ensemble var) (Γ : var) (FVs : list var) x y v v'  :
+    FV_inv k j GII GI b rho1 H1 rho2 H2 c Scope Funs Γ FVs ->
+    ~ x \in (FromList FVs \\ (Scope :|: Funs)) ->
+    y <> Γ ->
+    FV_inv k j GII GI b (M.set x v rho1) H1 (M.set y v' rho2) H2 c Scope Funs Γ FVs.
+  Proof.
+    intros. eapply FV_inv_set_not_in_FVs_r; eauto.
+    eapply FV_inv_set_not_in_FVs_l; eauto.
+  Qed.
+  
+
+  (** [Fun_inv] is heap monotonic  *)
+  Lemma FV_inv_heap_mon (k j : nat) (GII : GIInv) (GI : GInv) (b : Inj)
+        (rho1 : env) (H1 H1' : heap block) (rho2 : env) (H2 H2' : heap block)
+        (c : cTag) (Scope Funs : Ensemble var) (Γ : var) (FVs : list var) :
+    well_formed (reach' H1 (env_locs rho1 (FromList FVs \\ (Scope :|: Funs)))) H1 ->
+    well_formed (reach' H2 (env_locs rho2 [set Γ])) H2 ->
+    env_locs rho1 (FromList FVs \\ (Scope :|: Funs)) \subset dom H1 ->
+    env_locs rho2 [set Γ] \subset dom H2 ->
+    H1 ⊑ H1' ->
+    H2 ⊑ H2' ->
+    FV_inv k j GII GI b rho1 H1 rho2 H2 c Scope Funs Γ FVs ->
+    FV_inv k j GII GI b rho1 H1' rho2 H2' c Scope Funs Γ FVs.
+  Proof.
+    intros Hw1 Hw2 He1 He2 Hs1 Hs2.
+    intros (x1 & x2 & Hget1 & Hget2 & Hall).
+    repeat eexists; eauto.
+    eapply Forall2_P_monotonic_strong; [| eassumption ].
+    intros y1 v2 Hin1 Hin2 Hp [v1 [Hget3 Hrel]].
+    eexists; split; eauto. 
+    eapply cc_approx_val_heap_monotonic; try eassumption.
+    eapply well_formed_antimon; [| eassumption ].
+    eapply reach'_set_monotonic.
+    eapply Included_trans;
+      [| eapply env_locs_monotonic; eapply Singleton_Included ].
+    rewrite env_locs_Singleton; eauto. reflexivity.
+    now constructor; eauto.
+    eapply well_formed_antimon; [| eassumption ].
+    rewrite (reach_unfold H2 (env_locs rho2 [set Γ])).
+    eapply Included_Union_preserv_r.
+    eapply reach'_set_monotonic.
+    rewrite env_locs_Singleton; eauto.
+    simpl. rewrite post_Singleton; eauto.
+    eapply In_Union_list. eapply in_map.
+    eassumption.
+    eapply Included_trans; [| eassumption ].
+    eapply Included_trans; [| eapply env_locs_monotonic; eapply Singleton_Included ].
+    rewrite env_locs_Singleton; eauto. reflexivity.
+    now constructor; eauto.
+    eapply Included_trans; [| eapply reachable_in_dom; eassumption ].
+    rewrite (reach_unfold H2 (env_locs rho2 [set Γ])).
+    eapply Included_Union_preserv_r.
+    eapply Included_trans; [| eapply reach'_extensive ].
+    rewrite env_locs_Singleton; eauto.
+    simpl. rewrite post_Singleton; eauto.
+    eapply In_Union_list. eapply in_map.
+    eassumption.
+  Qed.
+
+  (** [Fun_inv] under rename extension  *)
+  Lemma FV_inv_rename_ext (k j : nat) (GII : GIInv) (GI : GInv) (b b' : Inj)
+        (rho1 : env) (H1 H2 : heap block) (rho2 : env) 
+        (c : cTag) (Scope Funs : Ensemble var) (Γ : var) (FVs : list var) :
+    FV_inv k j GII GI b rho1 H1 rho2 H2 c Scope Funs Γ FVs ->
+    f_eq_subdomain (reach' H1 (env_locs rho1 (FromList FVs \\ (Funs :|: Scope)))) b' b ->
+    FV_inv k j GII GI b' rho1 H1 rho2 H2 c Scope Funs Γ FVs.
+  Proof.
+    intros (x1 & x2 & Hget1 & Hget2 & Hall) Hfeq.
+    repeat eexists; eauto.
+    eapply Forall2_P_monotonic_strong; [| eassumption ].
+    intros y1 v2 Hin1 Hin2 Hp [v1 [Hget3 Hrel]].
+    eexists; split; eauto.
+    eapply cc_approx_val_rename_ext; try eassumption.
+    eapply f_eq_subdomain_antimon; try eassumption.
+    eapply reach'_set_monotonic.
+    eapply get_In_env_locs; eauto.
+    constructor; eauto. rewrite Union_commut. eassumption.
+  Qed.
+
+
+  (** [Fun_inv] monotonic *)
+  Lemma FV_inv_Scope_mon (k j : nat) (GII : GIInv) (GI : GInv) (b : Inj)
+        (rho1 : env) (H1 H2 : heap block) (rho2 : env) 
+        (c : cTag) (Scope Scope' Funs : Ensemble var) (Γ : var) (FVs : list var) :
+    FV_inv k j GII GI b rho1 H1 rho2 H2 c Scope Funs Γ FVs ->
+    Scope \subset Scope' -> 
+    FV_inv k j GII GI b rho1 H1 rho2 H2 c Scope' Funs Γ FVs.
+  Proof.
+    intros (x1 & x2 & Hget1 & Hget2 & Hall) Hfeq.
+    repeat eexists; eauto. eapply Forall2_P_monotonic. eassumption.
+    now eauto with Ensembles_DB. 
+  Qed.
+
+  Lemma FV_inv_Funs_mon (k j : nat) (GII : GIInv) (GI : GInv) (b : Inj)
+        (rho1 : env) (H1 H2 : heap block) (rho2 : env) 
+        (c : cTag) (Scope Funs Funs' : Ensemble var) (Γ : var) (FVs : list var) :
+    FV_inv k j GII GI b rho1 H1 rho2 H2 c Scope Funs Γ FVs ->
+    Funs \subset Funs' -> 
+    FV_inv k j GII GI b rho1 H1 rho2 H2 c Scope Funs' Γ FVs.
+  Proof.
+    intros (x1 & x2 & Hget1 & Hget2 & Hall) Hfeq.
+    repeat eexists; eauto. eapply Forall2_P_monotonic. eassumption.
+    now eauto with Ensembles_DB. 
+  Qed.
+  
+  (** * Lemmas about [Fun_inv] *)
   Lemma Fun_inv_image_post (k j : nat) (GII : GIInv) (GI : GInv) (b : Inj)
              (rho1 : env) (H1 : heap block) (rho2 : env) (H2 : heap block)
              (Scope Funs : Ensemble var) (σ : var -> var) :
     Fun_inv k j GII GI b rho1 H1 rho2 H2 Scope Funs σ ->
-    image b ((post H1 ^ j) (env_locs rho1 Funs)) <-->
-          (post H2 ^ j) (env_locs rho2 (image σ Funs)).
+    image b ((post H1 ^ j) (env_locs rho1 (Funs \\ Scope))) <-->
+          (post H2 ^ j) (env_locs rho2 (image σ (Funs \\ Scope))).
   Proof.
     intros Hfun. split.
     - intros l [l' [Hin Heq]]. subst.
       edestruct post_n_exists_Singleton as [l'' [Hpost' Hin']]; eauto.
-      edestruct Hpost' as [f [Hinf Hgetf]].
-      edestruct Hfun as (lf1 & lf2 & Hget1 & Hget2 & Hrel); eauto. 
+      edestruct Hpost' as [f [Hinf Hgetf]]. inv Hinf.
+      edestruct Hfun as (lf1 & lf2 & Hget1 & Hget2 & Hrel); eauto.
       rewrite Hget1 in Hgetf.
       eapply cc_approx_val_image_eq in Hrel.
       eapply post_n_set_monotonic.
       eapply env_locs_monotonic.
-      eapply Singleton_Included. eexists; split; eauto.
+      eapply Singleton_Included. eexists; split; eauto. constructor; eauto.
       eapply post_n_set_monotonic. eapply env_locs_Singleton; eauto.
       eapply Hrel. eexists; split;  eauto.
       eapply post_n_set_monotonic; eauto. eapply Singleton_Included. eassumption.
     - intros l Hpost.
       edestruct post_n_exists_Singleton as [l'' [Hpost' Hin']]; eauto.
       edestruct Hpost' as [f' [[f'' [Hinf' Heq]] Hgetf]]; subst.
+      inv Hinf'.
       edestruct Hfun as (lf1 & lf2 & Hget1 & Hget2 & Hrel); eauto.
-      eapply cc_approx_val_image_eq in Hrel.
+       eapply cc_approx_val_image_eq in Hrel.
       rewrite Hget2 in Hgetf. destruct lf2; inv Hgetf. eapply Hrel in Hin'.
       eapply image_monotonic; eauto.
-      eapply post_n_set_monotonic. eexists; split; eauto.
+      eapply post_n_set_monotonic. eexists; split; eauto. constructor; eauto.
       rewrite Hget1; eauto.
   Qed.
-
+  
   Lemma Fun_inv_j_monotonic (k j' j : nat) (GII : GIInv) (GI : GInv) (b : Inj)
         (rho1 : env) (H1 : heap block) (rho2 : env) (H2 : heap block)
         (Scope Funs : Ensemble var) (σ : var -> var) :
@@ -193,32 +467,72 @@ Module ClosureConversionCorrect (H : Heap).
     j' <= j ->
     Fun_inv k j' GII GI b rho1 H1 rho2 H2 Scope Funs σ .
   Proof.
-    intros Hfv Hlt f Hin'.
+    intros Hfv Hlt f Hin' Hin''.
     edestruct Hfv as (lf1 & lf2 & Hget1 & Hget2 & Hrel); eauto.
     repeat eexists; eauto.
     eapply cc_approx_val_j_monotonic; eauto.
   Qed.
+  
+  Lemma Fun_inv_monotonic (k k' j : nat) (GII : GIInv) (GI : GInv) (b : Inj)
+        (rho1 : env) (H1 : heap block) (rho2 : env) (H2 : heap block)
+        (Scope Funs : Ensemble var) (σ : var -> var) :
+    Fun_inv k j GII GI b rho1 H1 rho2 H2 Scope Funs σ  ->
+    k' <= k ->
+    Fun_inv k' j GII GI b rho1 H1 rho2 H2 Scope Funs σ .
+  Proof.
+    intros Hfv Hlt f Hin' Hin''.
+    edestruct Hfv as (lf1 & lf2 & Hget1 & Hget2 & Hrel); eauto.
+    repeat eexists; eauto.
+    eapply cc_approx_val_monotonic; eauto.
+  Qed.
 
+  Lemma Fun_inv_set_not_in_Funs_l (k  j : nat) (GII : GIInv) (GI : GInv) (b : Inj)
+        (rho1 : env) (H1 : heap block) (rho2 : env) (H2 : heap block)
+        (Scope Funs : Ensemble var) (σ : var -> var) x v :
+    Fun_inv k j GII GI b rho1 H1 rho2 H2 Scope Funs σ  ->
+    ~ x \in (Funs \\ Scope) ->
+    Fun_inv k j GII GI b (M.set x v rho1) H1 rho2 H2 Scope Funs σ .
+  Proof.
+    intros Hfv Hlt f Hnin Hin.
+    edestruct Hfv as (lf1 & lf2 & Hget1 & Hget2 & Hrel); eauto.
+    repeat eexists; eauto.
+    rewrite M.gso; eauto. intros Hc; inv Hc; eauto.
+    eapply Hlt; constructor; eauto.
+  Qed.
+  
   Lemma Fun_inv_set_not_in_Funs_r (k  j : nat) (GII : GIInv) (GI : GInv) (b : Inj)
         (rho1 : env) (H1 : heap block) (rho2 : env) (H2 : heap block)
         (Scope Funs : Ensemble var) (σ : var -> var) x v :
     Fun_inv k j GII GI b rho1 H1 rho2 H2 Scope Funs σ  ->
-    ~ x \in (image σ Funs) ->
+    ~ x \in (image σ (Funs \\ Scope)) ->
     Fun_inv k j GII GI b rho1 H1 (M.set x v rho2) H2 Scope Funs σ .
   Proof.
-    intros Hfv Hlt f Hin'.
+    intros Hfv Hlt f Hnin Hin.
     edestruct Hfv as (lf1 & lf2 & Hget1 & Hget2 & Hrel); eauto.
     repeat eexists; eauto.
     rewrite M.gso; eauto. intros Hc; inv Hc; eauto.
-    eapply Hlt; eexists; split; eauto.
+    eapply Hlt; eexists; split; eauto. constructor; eauto.
+  Qed.
+
+  Lemma Fun_inv_set_not_in_Funs (k  j : nat) (GII : GIInv) (GI : GInv) (b : Inj)
+        (rho1 : env) (H1 : heap block) (rho2 : env) (H2 : heap block)
+        (Scope Funs : Ensemble var) (σ : var -> var) x y v v' :
+    Fun_inv k j GII GI b rho1 H1 rho2 H2 Scope Funs σ  ->
+    ~ x \in (Funs \\ Scope) ->
+    ~ y \in image σ (Funs \\ Scope) ->
+    Fun_inv k j GII GI b (M.set x v rho1) H1 (M.set y v' rho2) H2 Scope Funs σ .
+  Proof.
+    intros Hfv Hnin Hnin'.
+    eapply Fun_inv_set_not_in_Funs_r; eauto.
+    eapply Fun_inv_set_not_in_Funs_l; eauto.
   Qed.
   
   Lemma Fun_inv_image_reach (k : nat) (GII : GIInv) (GI : GInv) (b : Inj)
              (rho1 : env) (H1 : heap block) (rho2 : env) (H2 : heap block)
              (Scope Funs : Ensemble var) (σ : var -> var) :
     (forall j, Fun_inv k j GII GI b rho1 H1 rho2 H2 Scope Funs σ) ->
-    image b (reach' H1 (env_locs rho1 Funs)) <-->
-    reach' H2 (env_locs rho2 (image σ Funs)).
+    image b (reach' H1 (env_locs rho1 (Funs \\ Scope))) <-->
+    reach' H2 (env_locs rho2 (image σ (Funs \\ Scope))).
   Proof.
     intros Hfv. split.
     - intros l' [l [[m [Hm Hr]] Hin]].
@@ -236,8 +550,8 @@ Module ClosureConversionCorrect (H : Heap).
         (rho1 : env) (H1 : heap block) (rho2 : env) (H2 : heap block)
         (Scope Funs : Ensemble var) (σ : var -> var) :
     Fun_inv k j GII GI b rho1 H1 rho2 H2 Scope Funs σ ->
-    image b (reach_n H1 j (env_locs rho1 Funs)) <-->
-    (reach_n H2 j) (env_locs rho2 (image σ Funs)).
+    image b (reach_n H1 j (env_locs rho1 (Funs \\ Scope))) <-->
+    (reach_n H2 j) (env_locs rho2 (image σ (Funs \\ Scope))).
   Proof.
     intros Hfv. split.
     - intros l' [l [[m [Hm Hr]] Hin]].
@@ -250,7 +564,7 @@ Module ClosureConversionCorrect (H : Heap).
       destruct Hr as [l [Heql Hin]]. eexists; split; eauto.
       eexists; split; eauto.
   Qed.
-
+  
   Lemma Fun_inv_weak_in_Fun_inv k j P1 P2 rho1 H1 rho2 H2 β Scope Funs σ :
     Fun_inv k j P1 P2 β rho1 H1 rho2 H2 Scope Funs σ  ->
     Fun_inv_weak rho1 H1 rho2 H2 Scope Funs σ.
@@ -258,6 +572,64 @@ Module ClosureConversionCorrect (H : Heap).
     now firstorder. 
   Qed.
 
+  (** [Fun_inv] is heap monotonic  *)
+  Lemma Fun_inv_heap_mon (k  j : nat) (GII : GIInv) (GI : GInv) (b : Inj)
+        (rho1 : env) (H1 H1' : heap block) (rho2 : env) (H2 H2' : heap block)
+        (Scope Funs : Ensemble var) (σ : var -> var) :
+    well_formed (reach' H1 (env_locs rho1 (Funs \\ Scope))) H1 ->
+    well_formed (reach' H2 (env_locs rho2 (image σ (Funs \\ Scope)))) H2 ->
+    env_locs rho1 (Funs \\ Scope) \subset dom H1 ->
+    env_locs rho2 (image σ (Funs \\ Scope)) \subset dom H2 ->
+    H1 ⊑ H1' ->
+    H2 ⊑ H2' ->
+    Fun_inv k j GII GI b rho1 H1 rho2 H2 Scope Funs σ  ->
+    Fun_inv k j GII GI b rho1 H1' rho2 H2' Scope Funs σ.
+  Proof.
+    intros Hw1 Hw2 He1 He2 Hs1 Hs2 Hfv x Hnin Hin.
+    edestruct Hfv as (lf1 & lf2 & Hget1 & Hget2 & Hrel); eauto.
+    repeat eexists; eauto.
+    eapply cc_approx_val_heap_monotonic; try eassumption.
+    eapply well_formed_antimon; [| eassumption ].
+    eapply reach'_set_monotonic. eapply get_In_env_locs; eauto.
+    now constructor; eauto.
+    eapply well_formed_antimon; [| eassumption ].
+    eapply reach'_set_monotonic. eapply get_In_env_locs; eauto.
+    eexists; split; auto. constructor; eauto.
+    eapply Included_trans; [| eassumption ]. eapply get_In_env_locs; eauto.
+    now constructor; eauto.
+    eapply Included_trans; [| eassumption ]. eapply get_In_env_locs; eauto.
+    eexists; split; auto.
+    now constructor; eauto.
+  Qed.
+
+
+  (** [Fun_inv] under renaming extension  *)
+  Lemma Fun_inv_rename_ext (k  j : nat) (GII : GIInv) (GI : GInv) (b b' : Inj)
+        (rho1 : env) (H1  : heap block) (rho2 : env) (H2 : heap block)
+        (Scope Funs : Ensemble var) (σ : var -> var) :
+    Fun_inv k j GII GI b rho1 H1 rho2 H2 Scope Funs σ  ->
+    f_eq_subdomain (reach' H1 (env_locs rho1 (Funs \\ Scope))) b' b ->
+    Fun_inv k j GII GI b' rho1 H1 rho2 H2 Scope Funs σ.
+  Proof.
+    intros Hfv Hfeq f Hnin Hin.
+    edestruct Hfv as (lf1 & lf2 & Hget1 & Hget2 & Hrel); eauto.
+    repeat eexists; eauto.
+    eapply cc_approx_val_rename_ext; try eassumption.
+    eapply f_eq_subdomain_antimon; [| eassumption ].
+    eapply reach'_set_monotonic.
+    eapply get_In_env_locs; eauto. constructor; eauto.
+  Qed.
+
+  (** [Fun_inv] monotonic *)
+  Lemma Fun_inv_Scope_mon (k j : nat) (GII : GIInv) (GI : GInv) (b : Inj)
+        (rho1 : env) (H1 H2 : heap block) (rho2 : env) 
+        (Scope Scope' Funs : Ensemble var) (σ : var -> var):
+    Fun_inv k j GII GI b rho1 H1 rho2 H2 Scope Funs σ ->
+    Scope \subset Scope' -> 
+    Fun_inv k j GII GI b rho1 H1 rho2 H2 Scope' Funs σ.
+  Proof.
+    now firstorder.
+  Qed.
 
   (** * Postcondition *)
   (** Enforces that the resource consumption of the target is within certain bounds *)
@@ -414,11 +786,27 @@ Module ClosureConversionCorrect (H : Heap).
       eapply Disjoint_sym. eapply Disjoint_Union_r. eassumption.
       intros Hc. eapply Hnin. eauto.
   Qed.        
-  
+
+  (* TODO move *)
+  Lemma Forall2_P_nthN (A B : Type) P (R : A -> B -> Prop) (l1 : list A) 
+        (l2 : list B) (n : N) (v1 : A): 
+    Forall2_P P R l1 l2 ->
+    nthN l1 n = Some v1 ->
+    ~ P v1 ->
+    exists v2 : B, nthN l2 n = Some v2 /\ R v1 v2.
+  Proof.
+    intros Hall; revert v1 n. induction Hall; intros v1 n Hnth Hall'.
+    - inv Hnth.
+    - destruct n.
+      + simpl in Hnth. inv Hnth.
+        eexists. split; simpl; eauto.
+      + edestruct IHHall as [v2 [Hnth2 Hr]]; eauto.
+  Qed.
+    
   Lemma project_var_ctx_to_heap_env Scope Funs σ c Γ FVs x x' C S S' v1 rho1 rho2 H1 H2:
     project_var Scope Funs σ c Γ FVs S x x' C S' ->
     Fun_inv_weak rho1 H1 rho2 H2 Scope Funs σ  ->
-    FV_inv_weak rho1 rho2 H2 c Γ FVs ->
+    FV_inv_weak rho1 rho2 H2 c Scope Funs Γ FVs ->
     M.get x rho1 = Some v1 ->
     exists H2' rho2' s, ctx_to_heap_env C H2 rho2 H2' rho2' s.
   Proof.
@@ -427,19 +815,19 @@ Module ClosureConversionCorrect (H : Heap).
     - edestruct HFun as
           (vf1 & vf4 & Hget1 & Hget2) ; eauto.
       repeat eexists; constructor; eauto.
-    - edestruct HFV as (v & vs & l & Hget1 & Hget2 & Hall).
-      edestruct (Forall2_nthN _ FVs vs N x Hall) as [v' [Hnth [v'' Hget'']]]; eauto.
-      repeat eexists. econstructor; eauto. constructor. 
+    - edestruct HFV as (v & vs  & Hget1 & Hget2 & Hall).
+      edestruct Forall2_P_nthN as [v2 [Hnth Hr]]; eauto. 
+      intros Hc; inv Hc; eauto.
+      repeat eexists. econstructor; eauto.
+      constructor.
   Qed.
   
   Lemma project_vars_ctx_to_heap_env Scope Funs σ c Γ FVs xs xs' C S S' vs1 rho1 H1 rho2 H2:
-    Disjoint _ S (Union var Scope
-                        (Union var (image σ Funs)
-                               (Union var (FromList FVs) (Singleton var Γ)))) ->
+    Disjoint _ S (FV_cc Scope Funs σ Γ) ->
     
     project_vars Scope Funs σ c Γ FVs S xs xs' C S' ->
     Fun_inv_weak rho1 H1 rho2 H2 Scope Funs σ ->
-    FV_inv_weak rho1 rho2 H2 c Γ FVs ->
+    FV_inv_weak rho1 rho2 H2 c Scope Funs Γ FVs ->
     getlist xs rho1 = Some vs1 ->
     exists H2' rho2' s, ctx_to_heap_env C H2 rho2 H2' rho2' s.
   Proof.
@@ -458,22 +846,22 @@ Module ClosureConversionCorrect (H : Heap).
       edestruct IHxs with (H2 := H2') (rho2 := rho2') as [H2'' [rho2'' [s' Hctx2]]]; [| eassumption | | | eassumption | ].
       + eapply Disjoint_Included_l; [| eassumption ].
         eapply project_var_free_set_Included. eassumption.
-      + intros f Hin.
+      + intros f Hin Hnin.
         edestruct HFun as (vf1 & vf2 & Hgetf1 & Hgetf2); try eassumption.
         repeat eexists; eauto.
         erewrite <- project_var_get; try eassumption.
         intros Hin'. eapply HD. constructor. now eauto.
-        right. left. eexists. split; eauto.
-      + edestruct HFV as [v' [vs [l' [Hget [Hget1 Hall]]]]]; eauto.
+        left. right. eexists. split; eauto. constructor; eauto.
+      + edestruct HFV as [v' [vs [Hget [Hget1 Hall]]]]; eauto.
         repeat eexists; eauto.
         * erewrite <- project_var_get; try eassumption.
           intros Hin'. eapply HD. constructor. now eauto.
-          right. right. right. reflexivity.
+          right. reflexivity.
         * erewrite ctx_to_heap_env_subheap. reflexivity.
           eassumption. eassumption.
       + exists H2'', rho2'', (s + s'). eapply ctx_to_heap_env_comp_ctx_f_r; eassumption.
   Qed.
-
+  
   (** [project_var] preserves env_locs in dom *)
   Lemma project_var_env_locs Scope Funs σ c Γ FVs x x' C S S' e k rho H rho' H':
     project_var Scope Funs σ c Γ FVs S x x' C S' ->
@@ -503,16 +891,22 @@ Module ClosureConversionCorrect (H : Heap).
   Lemma project_var_env_locs' Scope Funs σ c Γ FVs x x' C S S' k rho H rho' H':
     project_var Scope Funs σ c Γ FVs S x x' C S' ->
     ctx_to_heap_env C H rho H' rho' k ->
-    well_formed (reach' H (env_locs rho (Scope :|: (image σ Funs) :|: [set Γ]))) H ->
-    env_locs rho (Scope :|: (image σ Funs) :|: [set Γ]) \subset dom H ->
-    env_locs rho' (x' |: Scope :|: (image σ Funs) :|: [set Γ]) \subset dom  H'.
+    well_formed (reach' H (env_locs rho (FV_cc Scope Funs σ Γ))) H ->
+    env_locs rho (FV_cc Scope Funs σ Γ) \subset dom H ->
+    env_locs rho' (x' |: (FV_cc Scope Funs σ Γ)) \subset dom  H'.
   Proof with (now eauto with Ensembles_DB). 
+    unfold FV_cc. rewrite !Union_assoc.
     intros Hvar Hctx Hlocs Hwf. inv Hvar; inv Hctx.
-    - rewrite (Union_Same_set [set x']). eassumption.
+    - repeat rewrite (Union_Same_set [set x']) at 1. eassumption.
       eapply Singleton_Included; eauto.
-    - rewrite (Union_commut [set (σ x)]).
-      rewrite <- (Union_assoc Scope). rewrite (Union_Same_set [set _]). eassumption.
+    - rewrite (Union_commut [set (σ x)]) at 1.
+      rewrite <- (Union_assoc Scope). rewrite (Union_Same_set [set _]).
+      eapply Included_trans; [| eassumption ]. eapply env_locs_monotonic.
+      eapply Included_Union_compat; [| reflexivity ].
+      eapply Included_Union_compat. reflexivity.
+      eapply image_monotonic...
       eapply Singleton_Included; eauto. eexists; split; eauto.
+      split; eauto.
     - inv H18.
       eapply Included_trans. eapply env_locs_set_Inlcuded'.
       simpl. eapply Union_Included.
@@ -598,16 +992,18 @@ Module ClosureConversionCorrect (H : Heap).
   Lemma project_var_well_formed' Scope Funs σ c Γ FVs x x' C S S' k rho H rho' H':
     project_var Scope Funs σ c Γ FVs S x x' C S' ->
     ctx_to_heap_env C H rho H' rho' k ->
-    (env_locs rho (Scope :|: (image σ Funs) :|: [set Γ])) \subset dom H ->
-    well_formed (reach' H (env_locs rho (Scope :|: (image σ Funs) :|: [set Γ]))) H ->
-    well_formed (reach' H' (env_locs rho' (x' |: Scope :|: (image σ Funs) :|: [set Γ]))) H'.
+    (env_locs rho (FV_cc Scope Funs σ Γ)) \subset dom H ->
+    well_formed (reach' H (env_locs rho (FV_cc Scope Funs σ Γ))) H ->
+    well_formed (reach' H' (env_locs rho' (x' |: (FV_cc Scope Funs σ Γ)))) H'.
   Proof with (now eauto with Ensembles_DB). 
+    unfold FV_cc. rewrite !Union_assoc.
     intros Hvar Hctx Hlocs Hwf. inv Hvar; inv Hctx.
-    - simpl; eauto. rewrite (Union_Same_set [set x']). eassumption.
+    - simpl; eauto. rewrite (Union_Same_set [set x']).
+      eassumption.
       eapply Singleton_Included...
     - rewrite (Union_commut [set (σ x)]).
       rewrite <- (Union_assoc Scope). rewrite (Union_Same_set [set _]). eassumption.
-      eapply Singleton_Included; eauto. eexists; split; eauto.
+      eapply Singleton_Included; eauto. eexists; split; eauto. constructor; eauto.
     - inv H18.
       eapply well_formed_antimon; [| eapply well_formed_reach_set; try eassumption ].
       + eapply reach'_set_monotonic. eapply env_locs_monotonic.
@@ -634,7 +1030,7 @@ Module ClosureConversionCorrect (H : Heap).
     - inv H18. rewrite env_locs_set_not_In. reflexivity. 
       intros Hc; eapply HD; eauto.
   Qed.
-
+  
    Lemma project_vars_env_locs_subset Scope Funs σ c Γ FVs xs xs' C S S' S1 k rho H rho' H':
     project_vars Scope Funs σ c Γ FVs S xs xs' C S' ->
     ctx_to_heap_env C H rho H' rho' k ->
@@ -649,18 +1045,6 @@ Module ClosureConversionCorrect (H : Heap).
       rewrite project_var_env_locs_subset; eauto.
       reflexivity. eapply Disjoint_Included_r; try eassumption.
       eapply project_var_free_set_Included; eauto.
-  Qed.
-
-  Lemma project_var_not_In_free_set' Scope Funs σ c Γ FVs x x' C S S'  :
-    project_var Scope Funs σ c Γ FVs S x x' C S' ->
-    Disjoint _ S (Scope :|: (image σ Funs)) ->
-    ~ In _ S' x'.
-  Proof.
-    intros Hproj Hd. inv Hproj; intros Hc.
-    - eapply Hd. eauto.
-    - eapply Hd; eauto. constructor; eauto. right.
-      eexists; eauto.
-    - inv Hc. exfalso. eauto.    
   Qed.
 
   Lemma project_var_heap Scope Funs σ c Γ FVs x x' S S' C H rho H' rho' k :
@@ -707,10 +1091,10 @@ Module ClosureConversionCorrect (H : Heap).
   Lemma project_vars_env_locs' Scope Funs σ c Γ FVs xs xs' C S S' k rho H rho' H':
     project_vars Scope Funs σ c Γ FVs S xs xs' C S' ->
     ctx_to_heap_env C H rho H' rho' k ->
-    Disjoint _ S (Scope :|: (image σ Funs)) ->
-    well_formed (reach' H (env_locs rho (Scope :|: (image σ Funs) :|: [set Γ]))) H ->
-    env_locs rho (Scope :|: (image σ Funs) :|: [set Γ]) \subset dom H ->
-    env_locs rho' (FromList xs' :|: Scope :|: (image σ Funs) :|: [set Γ]) \subset dom  H'.
+    Disjoint _ S (Scope :|: (image σ (Funs \\ Scope))) ->
+    well_formed (reach' H (env_locs rho (FV_cc Scope Funs σ Γ))) H ->
+    env_locs rho (FV_cc Scope Funs σ Γ) \subset dom H ->
+    env_locs rho' (FromList xs' :|: (FV_cc Scope Funs σ Γ)) \subset dom  H'.
   Proof with (now eauto with Ensembles_DB). 
     intros Hvar. revert rho H rho' H' k. 
     induction Hvar; intros rho1 H1 rho2 H2 k Hctx Hd Hlocs Hwf.
@@ -726,7 +1110,7 @@ Module ClosureConversionCorrect (H : Heap).
       eapply env_locs_monotonic...
       eapply Disjoint_Singleton_l. eapply project_var_not_In_free_set'. eassumption.
       eapply Disjoint_Included_r; [| eassumption ]...
-      rewrite !Union_assoc. eapply IHHvar; eauto.
+      eapply IHHvar; eauto.
       eapply Disjoint_Included_l. eapply project_var_free_set_Included. eassumption.
       eassumption.
       eapply well_formed_antimon; [| eapply project_var_well_formed'; eauto ].
@@ -756,10 +1140,10 @@ Module ClosureConversionCorrect (H : Heap).
   Lemma project_vars_well_formed' Scope Funs σ c Γ FVs xs xs' C S S' k rho H rho' H':
     project_vars Scope Funs σ c Γ FVs S xs xs' C S' ->
     ctx_to_heap_env C H rho H' rho' k ->
-    Disjoint _ S (Scope :|: (image σ Funs)) ->
-    (env_locs rho (Scope :|: (image σ Funs) :|: [set Γ])) \subset dom H ->
-    well_formed (reach' H (env_locs rho (Scope :|: (image σ Funs) :|: [set Γ]))) H ->
-    well_formed (reach' H' (env_locs rho' (FromList xs' :|: Scope :|: (image σ Funs) :|: [set Γ]))) H'.
+    Disjoint _ S (Scope :|: (image σ (Funs \\ Scope))) ->
+    (env_locs rho (FV_cc Scope Funs σ Γ)) \subset dom H ->
+    well_formed (reach' H (env_locs rho (FV_cc Scope Funs σ Γ))) H ->
+    well_formed (reach' H' (env_locs rho' (FromList xs' :|: (FV_cc Scope Funs σ Γ)))) H'.
   Proof with (now eauto with Ensembles_DB). 
     intros Hvar. revert rho H rho' H' k. 
     induction Hvar; intros rho1 H1 rho2 H2 k Hctx HD Hlocs Hwf.
@@ -778,7 +1162,7 @@ Module ClosureConversionCorrect (H : Heap).
       eapply Disjoint_Singleton_l. eapply project_var_not_In_free_set'.
       eassumption.
       eapply Disjoint_Included_r; [| eassumption ]...
-      rewrite !Union_assoc. eapply IHHvar; eauto.
+      eapply IHHvar; eauto.
       eapply Disjoint_Included_l. eapply project_var_free_set_Included. eassumption.
       eassumption.
       eapply Included_trans; [| eapply project_var_env_locs'; eauto ].
@@ -786,125 +1170,6 @@ Module ClosureConversionCorrect (H : Heap).
       eapply well_formed_antimon; [| eapply project_var_well_formed'; eauto ].
       eapply reach'_set_monotonic. eapply env_locs_monotonic...
   Qed.
-
-  (** TODO move *)
-
-  Lemma cc_approx_val_image_reach_eq GIP GP (k : nat) (β : Inj)  (H1 H2 : heap block)
-        (v1 v2 : value) :
-    (forall j, (Res (v1, H1)) ≺ ^ (k ; j ; GIP ; GP ; β) (Res (v2, H2))) ->
-    image β (reach' H1 (val_loc v1)) <--> (reach' H2 (val_loc v2)).
-  Proof.
-    intros Hres. split.
-    - intros l' [l [[m [Hm Hr]] Hin]].
-      eapply cc_approx_val_image_eq in Hres. eexists m.
-      split; eauto. eapply Hres. eexists. split; eauto.
-    - intros l' [m [Hm Hr]].
-      eapply cc_approx_val_image_eq in Hres. eapply Hres in Hr.
-      destruct Hr as [l [Heql Hin]]. eexists; split; eauto.
-      eexists; split; eauto.
-  Qed.
-  
-  Lemma cc_approx_env_image_reach_eq GIP GP
-        (k : nat) (β : Inj)
-        (H1 H2 : heap block) (rho1 rho2 : env) (x y : var) (v : value) :
-    (forall j, cc_approx_var_env k j GIP GP β H1 rho1 H2 rho2 x y) ->
-    M.get x rho1 = Some v -> 
-    image β (reach' H1 (env_locs rho1 [set x])) <-->
-    reach' H2 (env_locs rho2 [set y]).
-  Proof.
-    intros Hcc Hget.
-    edestruct (Hcc 0) as [v' [Hget' Hv]]; eauto.
-    rewrite !env_locs_Singleton; eauto. 
-    rewrite cc_approx_val_image_reach_eq. reflexivity.
-    intros j; eauto.
-    edestruct (Hcc j) as [v'' [Hget'' Hv']]; eauto.
-    repeat subst_exp. eassumption.
-  Qed.
-
-  Lemma cc_approx_env_image_eq GIP GP S (k j : nat) (β : Inj)
-        (H1 H2 : heap block) (rho1 rho2 : env) :
-    (H1, rho1) ⋞ ^ (S; k; j; GIP; GP; β) (H2, rho2) ->
-    binding_in_map S rho1 ->
-    image β ((post H1 ^ j) (env_locs rho1 S)) <--> (post H2 ^ j) (env_locs rho2 S).
-  Proof.
-    intros Henv Hbin. split.
-    - intros l1 [l2 [Hin Hbeq]].
-      edestruct post_n_exists_Singleton as [l' [Henv' Hp]]. eassumption.
-      destruct Henv' as [x [Hgetx Hinx]].
-      destruct (M.get x rho1) eqn:Hget1; try now inv Hinx.
-      destruct v; inv Hinx; try contradiction.
-      assert (Hget2 := Hget1).
-      eapply cc_approx_var_env_image_eq in Hget1; eauto.
-      eapply post_n_set_monotonic; [| eapply Hget1 ].
-      eapply env_locs_monotonic. now eapply Singleton_Included; eauto.
-      eexists; split; eauto.
-      eapply proper_post_n. eapply env_locs_Singleton. now eauto.
-      eassumption. 
-    - intros l Hp.
-      edestruct post_n_exists_Singleton as [l' [Henv' Hp']]. eassumption.
-      destruct Henv' as [x [Hgetx Hinx]].
-      destruct (M.get x rho2) eqn:Hget1; try now inv Hinx.
-      destruct v; inv Hinx; try contradiction.
-      eapply image_monotonic. eapply post_n_set_monotonic.
-      eapply env_locs_monotonic. eapply Singleton_Included. eassumption.
-      edestruct Hbin as [v Hget]; eauto.
-      edestruct Henv as [l'' [Hget' Hres]]; eauto. 
-      eapply cc_approx_var_env_image_eq; eauto.
-      eapply proper_post_n. now eapply env_locs_Singleton; eauto.
-      subst_exp. eassumption.
-  Qed.
-
-  Lemma cc_approx_env_image_reach_n GIP GP S (k j : nat) (β : Inj)
-        (H1 H2 : heap block) (rho1 rho2 : env) :
-    (H1, rho1) ⋞ ^ (S; k; j; GIP; GP; β) (H2, rho2) ->
-    binding_in_map S rho1 ->
-    image β ((reach_n H1 j) (env_locs rho1 S)) <--> (reach_n H2 j) (env_locs rho2 S).
-  Proof.
-    intros Hres HB. split.
-    - intros l' [l [[m [Hm Hr]] Hin]].
-      eapply cc_approx_env_P_j_monotonic in Hres; eauto. 
-      eapply cc_approx_env_image_eq in Hres. eexists m.
-      split; eauto. eapply Hres. eexists. split; eauto.
-      eassumption.
-    - intros l' [m [Hm Hr]].
-      eapply cc_approx_env_P_j_monotonic in Hres; eauto. 
-      eapply cc_approx_env_image_eq in Hres. eapply Hres in Hr.
-      destruct Hr as [l [Heql Hin]]. eexists; split; eauto.
-      eexists; split; eauto. eassumption.
-  Qed.
-
-  Lemma cc_approx_env_image_reach GIP GP S (k : nat) (β : Inj)
-        (H1 H2 : heap block) (rho1 rho2 : env) :
-    (forall j, (H1, rho1) ⋞ ^ (S; k; j; GIP; GP; β) (H2, rho2)) ->
-    binding_in_map S rho1 ->
-    image β (reach' H1 (env_locs rho1 S)) <--> reach' H2 (env_locs rho2 S).
-  Proof.
-    intros Hres HB. split.
-    - intros l' [l [[m [Hm Hr]] Hin]].
-      eapply cc_approx_env_P_j_monotonic in Hres; eauto. 
-      eapply cc_approx_env_image_eq in Hres. eexists m.
-      split; eauto. eapply Hres. eexists. split; eauto.
-      eassumption.
-    - intros l' [m [Hm Hr]].
-      eapply cc_approx_env_P_j_monotonic in Hres; eauto. 
-      eapply cc_approx_env_image_eq in Hres. eapply Hres in Hr.
-      destruct Hr as [l [Heql Hin]]. eexists; split; eauto.
-      eexists; split; eauto. eassumption.
-  Qed.
-
-  (* TODO move *)
-
-  Lemma cc_approx_var_env_set_neq_r GIP GP b :
-    forall (k j : nat)  (rho1 rho2 : env) (H1 H2 : heap block)
-      (y1 x2 y2 : var) ( v2 : value),
-      cc_approx_var_env k j GIP GP b H1 rho1 H2 rho2 y1 y2 ->
-      y2 <> x2 ->
-      cc_approx_var_env k j GIP GP b H1 rho1 H2 (M.set x2 v2 rho2) y1 y2.
-  Proof. 
-    intros k j rho1 rho2 H1 H2 x2 y1 y2 v2 Hval Hneq x' Hget.
-    rewrite M.gso in *; eauto.
-  Qed.
-
 
   Lemma project_var_preserves_cc_approx GII GI k j H1 rho1 H2 rho2 H2' rho2' b
         Scope Funs σ c Γ FVs x x' C S S' m y y' :
@@ -946,60 +1211,55 @@ Module ClosureConversionCorrect (H : Heap).
     
     (forall j, (H1, rho1) ⋞ ^ (Scope; k; j; GII; GI; b) (H2, rho2)) ->
     (forall j, Fun_inv k j GII GI b rho1 H1 rho2 H2 Scope Funs σ) ->
-    (forall j, FV_inv k j GII GI b rho1 H1 rho2 H2 c Γ FVs) ->
+    (forall j, FV_inv k j GII GI b rho1 H1 rho2 H2 c Scope Funs Γ FVs) ->
 
     ctx_to_heap_env C H2 rho2 H2' rho2' m ->
-
-    injective_subdomain (reach' H1 (env_locs rho1 (Scope :|: FromList FVs :|: Funs))) b ->
     
     binding_in_map Scope rho1 ->
-    Disjoint _ S (Scope :|: (image σ Funs) :|: (FromList FVs) :|: [set Γ]) ->
+    Disjoint _ S (FV_cc Scope Funs σ Γ) ->
 
     ~ In _ S' x' /\
-    injective_subdomain (reach' H1 (env_locs rho1 (x |: Scope :|: FromList FVs :|: Funs))) b /\
     (forall j, (H1, rho1) ⋞ ^ (Scope; k; j; GII; GI; b) (H2', rho2'))  /\
     (forall j, Fun_inv k j GII GI b rho1 H1 rho2' H2' Scope Funs σ) /\
-    (forall j, FV_inv k j GII GI b rho1 H1 rho2' H2' c Γ FVs) /\
+    (forall j, FV_inv k j GII GI b rho1 H1 rho2' H2' c Scope Funs Γ FVs) /\
     (forall j, cc_approx_var_env k j GII GI b H1 rho1 H2' rho2' x x').
+
   Proof with (now eauto with Ensembles_DB).
-    intros Hproj Hcc Hfun Henv Hctx Hinj Hbin Hd.
+    intros Hproj Hcc Hfun Henv Hctx Hbin Hd.
     inv Hproj.
-    - inv Hctx. split. intros Hc. eapply Hd; eauto.
-      split; [| split; [| split ; [| split ]]]; eauto.
-      rewrite (Union_Same_set [set x'])... intros j; eapply Hcc. eassumption.
+    - inv Hctx. split. intros Hc. eapply Hd; eauto. constructor; eauto. left; eauto.
+      split; [| split; [| split ]]; eauto.
+      intros j; eapply Hcc. eassumption.
     - inv Hctx.
-      split; [| split; [| split; [| split; [| split ]]]]. repeat split.
+      split; [| split; [| split; [| split ]]]. repeat split.
       + intros Hc. eapply Hd. constructor; eauto.
-        left. left. right. eexists; split; eauto.
-      + rewrite <- !Union_assoc, (Union_commut [set x]), <- !Union_assoc, (Union_commut _ [set x]).
-        rewrite (Union_Same_set [set x]). rewrite !Union_assoc.  eassumption.
-        eapply Singleton_Included; eauto.
+        left. right. eexists; split; eauto. constructor; eauto.
       + intros j. eapply Hcc; eauto.
       + eassumption.
       + eassumption.
       + intros j. edestruct (Hfun j) as (vf1 & vf2 & Hget1 & Hget2 & Hcc'); eauto.
         intros v1 Hget1'. repeat subst_exp. eexists; split; eauto.
     - inv Hctx. inv H19.
-      split; [| split; [| split; [| split; [| split ]]]]. repeat split.
+      split; [| split; [| split; [| split ]]]. repeat split.
       + intros Hc. inv Hc. eauto.
-      + rewrite (Union_commut [set x]), <- (Union_assoc _ _ (FromList FVs)).
-        rewrite (Union_Same_set [set x]). eassumption.
-        eapply Singleton_Included; eauto. eapply nthN_In; eauto.
       + intros j. eapply cc_approx_env_P_set_not_in_P_r. now eauto.
-        intros Hc. eapply Hd; eauto.
+        intros Hc. eapply Hd; eauto. constructor; eauto.
+        left; eauto.
       + intros j. eapply Fun_inv_set_not_in_Funs_r; eauto.
         intros Hc; eapply Hd. constructor; eauto.
+        constructor; eauto.
       + intros h. 
-        edestruct Henv as (v1 & vs1 & l' & Hget1 & Hget2 & Hall).
+        edestruct Henv as (v1 & vs1 & Hget1 & Hget2 & Hall).
         repeat eexists; eauto. 
         rewrite M.gso; eauto. intros Heq; subst. eapply Hd. constructor; eauto.
+        right. reflexivity.
       + intros j v' Hget.
-        edestruct (Henv j) as (v1 & vs1 & l' & Hget1 & Hget2 & Hall).
+        edestruct (Henv j) as (v1 & vs1 & Hget1 & Hget2 & Hall).
         eexists. rewrite M.gss. split. reflexivity.
-        edestruct (Forall2_nthN _ FVs vs1 N _ Hall H3) as (v2 & Hnth' & vs4 & Hget4 & Hrel).
-        repeat subst_exp. eassumption.
+        edestruct (Forall2_P_nthN _ _ _ _ FVs _ N _ Hall H3) as (v2 & Hnth' & vs4 & Hget4 & Hrel).
+        intros Hc; inv Hc; eauto. repeat subst_exp. eassumption.
   Qed.
-
+  
   Lemma project_var_setminus_same  Scope Funs σ c Γ FVs x x' C S S' : 
     project_var Scope Funs σ c Γ FVs S x x' C S' ->
     project_var Scope (Funs \\ Scope) σ c Γ FVs S x x' C S'.
@@ -1023,67 +1283,109 @@ Module ClosureConversionCorrect (H : Heap).
     
     (forall j, (H1, rho1) ⋞ ^ (Scope; k; j; GII; GI; b) (H2, rho2)) ->
     (forall j, Fun_inv k j GII GI b rho1 H1 rho2 H2 Scope Funs σ) ->
-    (forall j, FV_inv k j GII GI b rho1 H1 rho2 H2 c Γ FVs) ->
+    (forall j, FV_inv k j GII GI b rho1 H1 rho2 H2 c Scope Funs Γ FVs) ->
 
     ctx_to_heap_env C H2 rho2 H2' rho2' m ->
 
-    injective_subdomain (reach' H1 (env_locs rho1 (Scope :|: FromList FVs :|: Funs))) b ->
-    
     binding_in_map Scope rho1 -> 
-    Disjoint _ S (Scope :|: (image σ Funs) :|: (FromList FVs) :|: [set Γ]) ->
+    Disjoint _ S (FV_cc Scope Funs σ Γ) ->
 
     Disjoint _ (FromList xs') S' /\
-    injective_subdomain (reach' H1 (env_locs rho1 ((FromList xs) :|: Scope :|: FromList FVs :|: Funs))) b /\
     (forall j, (H1, rho1) ⋞ ^ (Scope; k; j; GII; GI; b) (H2', rho2'))  /\
     (forall j, Fun_inv k j GII GI b rho1 H1 rho2' H2' Scope Funs σ) /\
-    (forall j, FV_inv k j GII GI b rho1 H1 rho2' H2' c Γ FVs) /\
+    (forall j, FV_inv k j GII GI b rho1 H1 rho2' H2' c Scope Funs Γ FVs) /\
     (forall j, Forall2 (fun x x' => cc_approx_var_env k j GII GI b H1 rho1 H2' rho2' x x') xs xs').
   Proof with (now eauto with Ensembles_DB).
     intros Hvars. revert m H1 rho1 H2 rho2 H2' rho2'.
-    induction Hvars; intros m H1 rho1 H2 rho2 H2' rho2' Hcc Hfun Hfv Hctx Hinj Hb Hd. 
+    induction Hvars; intros m H1 rho1 H2 rho2 H2' rho2' Hcc Hfun Hfv Hctx Hb Hd. 
     - inv Hctx. split; [| split; [| split ; [| split ]]]; eauto.
       rewrite FromList_nil...
-      rewrite FromList_nil. rewrite Union_Empty_set_neut_l...
     - rewrite FromList_cons in *. 
       edestruct ctx_to_heap_env_comp_ctx_f_l as [rho3 [H3 [m1 [m2 [Hctx2 [Hctx3 Heq]]]]]].
       subst.
       eassumption. subst.
-      edestruct project_var_correct as (Hd' & Hinj' & Hcc' & Hfun' & Hfv' & Hall');
+      edestruct project_var_correct as (Hd' & Hcc' & Hfun' & Hfv' & Hall');
         try eassumption.
-      edestruct IHHvars as (Hd'' & Hinj'' & Hcc'' & Hfun'' & Hfv'' & Hall'');
+      edestruct IHHvars as (Hd'' & Hcc'' & Hfun'' & Hfv'' & Hall'');
       try eassumption.
       eapply Disjoint_Included_l; [| eassumption ].
       eapply project_var_free_set_Included. eassumption.
-      split; [| split; [| split ; [| split; [| split ] ]]]; eauto.
+      split; [| split; [| split ; [| split ]]]; eauto.
       * eapply Union_Disjoint_l. 
         eapply Disjoint_Included_r.
         eapply project_vars_free_set_Included. eassumption.
         eapply Disjoint_Singleton_l.
-        eapply project_var_not_In_free_set. eassumption.
+        eapply project_var_not_In_free_set'. eassumption.
         eapply Disjoint_Included_r; [| eassumption ].
-        rewrite <- !Union_assoc. eapply Included_Union_compat. reflexivity.
-        eapply Included_Union_compat. eapply image_monotonic...
-        reflexivity.        
-        eapply Disjoint_sym. eapply project_vars_not_In_free_set. eassumption.
+        unfold FV_cc...
+        eapply Disjoint_sym. eapply project_vars_not_In_free_set'. eassumption.
         eapply Disjoint_Included_l.
         eapply project_var_free_set_Included. eassumption.
         eapply Disjoint_Included_r; [| eassumption ].
-        rewrite <- !Union_assoc. eapply Included_Union_compat. reflexivity.
-        eapply Included_Union_compat. eapply image_monotonic...
-        reflexivity.
-      * eapply injective_subdomain_antimon. now apply Hinj.
-        eapply reach'_set_monotonic. eapply env_locs_monotonic.
-        rewrite FromList_cons. rewrite <- !Union_assoc. eapply Union_Included.
-        eapply Singleton_Included. rewrite (Union_commut (FromList FVs)).
-        eapply project_var_In_Union. eassumption.
-        eapply Union_Included.  rewrite (Union_commut (FromList FVs)).
-        eapply project_vars_In_Union. eassumption.
-        now eauto with Ensembles_DB.
+        unfold FV_cc...
       * intros j. constructor; eauto .
         eapply project_vars_preserves_cc_approx; eauto.
   Qed.
-  
 
+  (** [project_var] preserves injectiveness *)
+  Lemma project_var_same_set
+        Scope Funs σ c Γ FVs x x' C S S'  :
+    project_var Scope Funs σ c Γ FVs S x x' C S' ->
+    x |: (FV Scope Funs FVs) <--> FV Scope Funs FVs.
+  Proof with (now eauto with Ensembles_DB).
+    intros Hvar. rewrite Union_Same_set. reflexivity.
+    eapply Singleton_Included. eapply project_var_In_Union.
+    eassumption.
+  Qed.
+
+  Lemma project_vars_same_set
+        Scope Funs σ c Γ FVs x x' C S S'  :
+    project_vars Scope Funs σ c Γ FVs S x x' C S' ->
+    (FromList x) :|: (FV Scope Funs FVs) <--> FV Scope Funs FVs.
+  Proof with (now eauto with Ensembles_DB).
+    intros Hvar. rewrite Union_Same_set. reflexivity.
+    eapply project_vars_In_Union.
+    eassumption.
+  Qed.
+
+  Lemma image_FV GI GP k β H1 rho1 H2 rho2 Scope Funs FVs Γ σ c :
+    (forall j, (H1, rho1) ⋞ ^ (Scope ; k ; j ; GI ; GP ; β) (H2, rho2)) ->
+    (forall j, Fun_inv k j GI GP β rho1 H1 rho2 H2 Scope Funs σ) ->
+    (forall j, FV_inv k j GI GP β rho1 H1 rho2 H2 c Scope Funs Γ FVs) ->
+    binding_in_map Scope rho1 ->
+
+    (image β (reach' H1 (env_locs rho1 (FV Scope Funs FVs)))) \subset
+    reach' H2 ((env_locs rho2 (Scope :|: image σ (Funs \\ Scope))) :|: (post H2 (env_locs rho2 [set Γ]))).
+  Proof.
+    intros. unfold FV, FV_cc.
+    rewrite !env_locs_Union, !reach'_Union, !image_Union.
+    rewrite cc_approx_env_image_reach; try eassumption. 
+    rewrite Fun_inv_image_reach; try eassumption.
+    eapply Included_Union_compat. reflexivity.
+    eapply FV_inv_image_reach; try eassumption.
+  Qed.     
+
+  Lemma image_FV_eq GI GP k β H1 rho1 H2 rho2 Scope Funs FVs Γ σ c :
+    (forall j, (H1, rho1) ⋞ ^ (Scope ; k ; j ; GI ; GP ; β) (H2, rho2)) ->
+    (forall j, Fun_inv k j GI GP β rho1 H1 rho2 H2 Scope Funs σ) ->
+    (forall j, FV_inv k j GI GP β rho1 H1 rho2 H2 c Scope Funs Γ FVs) ->
+    binding_in_map Scope rho1 ->
+    Disjoint var (FromList FVs) (Scope :|: Funs) ->
+    (image β (reach' H1 (env_locs rho1 (FV Scope Funs FVs)))) <-->
+    reach' H2 ((env_locs rho2 (Scope :|: image σ (Funs \\ Scope))) :|: (post H2 (env_locs rho2 [set Γ]))).
+  Proof.
+    intros. unfold FV, FV_cc.
+    rewrite !env_locs_Union, !reach'_Union, !image_Union.
+    rewrite cc_approx_env_image_reach; try eassumption. 
+    rewrite Fun_inv_image_reach; try eassumption.
+    assert (Hd' := H5). eapply Setminus_Disjoint in H5.
+    eapply Same_set_Union_compat. reflexivity.
+    eapply Same_set_trans. eapply image_Proper_Same_set. (* ?????? *)
+    reflexivity. eapply Proper_reach'. reflexivity.
+    eapply Proper_env_locs. reflexivity. eassumption.
+    rewrite FV_inv_image_reach_eq; try eassumption. reflexivity.
+  Qed.     
+  
   (** Correctness of [Closure_conversion] *)
   Lemma Closure_conversion_correct (k : nat) (H1 H2 : heap block)
         (rho1 rho2 : env) (e1 e2 : exp) (C : exp_ctx)
@@ -1094,28 +1396,28 @@ Module ClosureConversionCorrect (H : Heap).
     (* [Fun] invariant *)
     (forall j, Fun_inv k j (Pre Hole_c) (Post 0) β rho1 H1 rho2 H2 Scope Funs σ) ->
     (* Free variables invariant *)
-    (forall j, FV_inv k j (Pre Hole_c) (Post 0) β rho1 H1 rho2 H2 c Γ FVs) ->
+    (forall j, FV_inv k j (Pre Hole_c) (Post 0) β rho1 H1 rho2 H2 c Scope Funs Γ FVs) ->
     (* location renaming is injective *)
     (* only needed to prove the lower bound *)
-    injective_subdomain (reach' H1 (env_locs rho1 (Scope :|: FromList FVs :|: Funs))) β ->
+    injective_subdomain (reach' H1 (env_locs rho1 (FV Scope Funs FVs))) β ->
     
     (* well-formedness *)
-    well_formed (reach' H1 (env_locs rho1 (Scope :|: Funs :|: FromList FVs))) H1 ->
-    (env_locs rho1 (Scope :|: Funs :|: FromList FVs)) \subset dom H1 ->
-    well_formed (reach' H2 (env_locs rho2 (Scope :|: (image σ Funs) :|: [set Γ]))) H2 ->
-    (env_locs rho2 (Scope :|:  (image σ Funs) :|: [set Γ])) \subset dom H2 ->
+    well_formed (reach' H1 (env_locs rho1 (FV Scope Funs FVs))) H1 ->
+    (env_locs rho1 (FV Scope Funs FVs)) \subset dom H1 ->
+    well_formed (reach' H2 (env_locs rho2 (FV_cc Scope Funs σ Γ))) H2 ->
+    (env_locs rho2 (FV_cc Scope Funs σ Γ)) \subset dom H2 ->
 
     
     (* [Γ] (the current environment parameter) is not bound in e *)
     ~ In _ (bound_var e1) Γ ->
     (* The free variables of e are defined in the environment *)
-    binding_in_map (Scope :|: Funs :|: FromList FVs) rho1 ->
+    binding_in_map (FV Scope Funs FVs) rho1 ->
     (* The blocks of functions have unique function names *)
     fundefs_names_unique e1 ->
     (* function renaming is injective in the [Funs] subdomain *)
     injective_subdomain Funs σ ->
     (* function renaming codomain is not shadowed by other vars *)
-    Disjoint _ (image σ Funs) (bound_var e1) ->
+    Disjoint _ (image σ (Funs \\ Scope)) (bound_var e1) ->
 
     
     (* [e'] is the closure conversion of [e] *)
@@ -1131,11 +1433,11 @@ Module ClosureConversionCorrect (H : Heap).
     - (* case Econstr *)
       assert (Hfv := Closure_conversion_pre_occurs_free_Included _ _ _ _ _ _ _ _ _ _ Hcc).
       assert (Hfv' := Closure_conversion_occurs_free_Included _ _ _ _ _ _ _ _ _ _ Hcc Hun).
-      rewrite !Union_assoc in Hfv'.
-
+      
       inv Hcc.
+
       edestruct (binding_in_map_getlist _ rho1 l Hbind) as [vl Hgetl].
-      rewrite <- Union_assoc. eapply project_vars_In_Union. eassumption.
+      eapply project_vars_In_Union. eassumption.
       
       edestruct project_vars_ctx_to_heap_env as [H2' [rho2' [m Hct]]]; try eassumption.
       specialize (Hfun 0); eapply Fun_inv_weak_in_Fun_inv; eassumption.
@@ -1147,13 +1449,13 @@ Module ClosureConversionCorrect (H : Heap).
       with (ILi := fun c => PostL c k H1 rho1 (Econstr v t l e1)) (II := fun C => Pre C k);
         [ now intros; eapply Post_transfer; eauto | now intros; eapply IP_ctx_to_heap_env; eauto
           | | | | | eassumption | ].
-
+      
       eapply well_formed_antimon. eapply reach'_set_monotonic. now eapply env_locs_monotonic; eauto.
       eassumption.
-
+      
       eapply well_formed_antimon. eapply reach'_set_monotonic. now eapply env_locs_monotonic; eauto.
       eassumption.
-
+      
       eapply Included_trans; [| eassumption ]. now eapply env_locs_monotonic; eauto.
       eapply Included_trans; [| eassumption ]. eapply env_locs_monotonic; eauto.
       
@@ -1161,13 +1463,14 @@ Module ClosureConversionCorrect (H : Heap).
       replace (comp_ctx_f Hole_c C) with C by eauto.
       assert (Hwf2' := Hwf2).
       assert (Hlocs2' := Hlocs2). 
-      eapply project_vars_well_formed' in Hwf2; try eassumption.
-      eapply project_vars_env_locs' in Hlocs2; try eassumption.
-
-      edestruct project_vars_correct as (Hd' & Hinj' & Henv' & Hfun' & HFVs' & Hvars);
+      eapply project_vars_well_formed' in Hwf2; try eassumption;
+      [| eapply Disjoint_Included_r; try eassumption; unfold FV_cc; now eauto with Ensembles_DB ].
+      eapply project_vars_env_locs' in Hlocs2; try eassumption;
+      [| eapply Disjoint_Included_r; try eassumption; unfold FV_cc; now eauto with Ensembles_DB ].
+      
+      edestruct project_vars_correct as (Hd' & Henv' & Hfun' & HFVs' & Hvars);
         try eassumption.
       eapply binding_in_map_antimon; [| eassumption ]...
-      rewrite <- !Union_assoc. eassumption.
       
       (* process Econstr one the right and left *)
       eapply cc_approx_exp_constr_compat 
@@ -1192,12 +1495,17 @@ Module ClosureConversionCorrect (H : Heap).
         eapply reach'_set_monotonic. eapply env_locs_monotonic. eassumption.
         eassumption.
       + admit. (* bounds -- find F *)
-      + (* Inductive case *) 
+      + (* Inductive case *)  
         intros vs1 vs2 l1 l2 H1' H2'' Hleq Ha1 Ha2 Hr1 Hr2 Hall j1.
-        (* monotonicity of the local invariant *)
+        (* monotonicity of the local invariant *) 
         eapply cc_approx_exp_rel_mon
         with (LP1 := PostL 0 (k - cost H1 rho1 (Econstr v t l e1)) H1' (M.set v (Loc l1) rho1) e1).
-        
+
+        assert (Hfeq : f_eq_subdomain (reach' H1 (env_locs rho1 (FV Scope Funs FVs))) β (β {l1 ~> l2})).
+                { eapply f_eq_subdomain_extend_not_In_S_r; [| reflexivity ].
+                  intros Hc. eapply reachable_in_dom in Hc.
+                  edestruct Hc as [vc Hgetc]. erewrite alloc_fresh in Hgetc; eauto. congruence.
+                  eassumption. eassumption. }
         (* Induction hypothesis *)
         { eapply IHk;
           [ | | | | | | | | | | | | now apply Hinj | | eassumption ].  
@@ -1206,14 +1514,16 @@ Module ClosureConversionCorrect (H : Heap).
               eapply cc_approx_env_set_alloc_Constr with (b := β {l1 ~> l2});
                 try eassumption.
               - eapply well_formed_antimon; [| eassumption ].
-                eapply reach'_set_monotonic. eapply env_locs_monotonic...
+                eapply reach'_set_monotonic. eapply env_locs_monotonic.
+                unfold FV...
               - eapply well_formed_antimon; [| eassumption ].
                 eapply reach'_set_monotonic. eapply env_locs_monotonic.
+                unfold FV_cc.
                 now eauto 20 with Ensembles_DB.
               - eapply Included_trans; [| eassumption ].
-                eapply env_locs_monotonic...
+                eapply env_locs_monotonic. unfold FV...
               - eapply Included_trans; [| eassumption ].
-                eapply env_locs_monotonic.
+                eapply env_locs_monotonic. unfold FV.
                 now eauto 20 with Ensembles_DB.
               - eapply well_formed_antimon. eapply reach'_set_monotonic.
                 eassumption.
@@ -1238,16 +1548,12 @@ Module ClosureConversionCorrect (H : Heap).
                 eapply cc_approx_env_P_antimon.
                 eapply cc_approx_env_P_monotonic. now eauto.
                 simpl in *; omega. now eauto with Ensembles_DB.
-                eapply f_eq_subdomain_extend_not_In_S_r; [| reflexivity ].
-                intros Hc. eapply reachable_in_dom in Hc.
-                edestruct Hc as [vc Hgetc]. erewrite alloc_fresh in Hgetc; eauto. congruence.
-                eapply well_formed_antimon; [| eassumption ].
+                eapply f_eq_subdomain_antimon; [| eassumption ].
                 eapply reach'_set_monotonic. eapply env_locs_monotonic...
-                eapply Included_trans; [| eassumption ]. eapply env_locs_monotonic...
               - rewrite extend_gss. reflexivity.
               - intros j3 Hlt3. eapply Forall2_monotonic_strong; [| now eapply Hall ].
                 intros x1 x2 Hin1 Hin2 Hrel. eapply cc_approx_val_rename_ext. now eapply Hrel.
-                assert (Hincl : val_loc x1 \subset env_locs rho1 (Scope :|: Funs :|: FromList FVs)).
+                assert (Hincl : val_loc x1 \subset env_locs rho1 (FV Scope Funs FVs)).
                 { eapply Included_trans; [| now eapply env_locs_monotonic; eauto ].
                   eapply Included_trans; [| eassumption ].
                   simpl. eapply In_Union_list. eapply in_map. eassumption. }
@@ -1262,20 +1568,64 @@ Module ClosureConversionCorrect (H : Heap).
                 eapply reach'_set_monotonic. eassumption.
 
                 eapply Included_trans; eassumption. }
-          * admit. (* fun inv env_set_alloc *)
-          * admit. (* FV inv env set alloc *)
+          * intros j'.
+            { eapply Fun_inv_set_not_in_Funs.
+              - eapply Fun_inv_heap_mon; try (now eapply HL.alloc_subheap; eauto).
+                + eapply well_formed_antimon; [| eassumption ].
+                  eapply reach'_set_monotonic. eapply env_locs_monotonic.
+                  unfold FV...
+                + eapply well_formed_antimon; [| eassumption ].
+                  eapply reach'_set_monotonic. eapply env_locs_monotonic.
+                  unfold FV_cc. now eauto 20 with Ensembles_DB.
+                + eapply Included_trans; [| eassumption ].
+                  eapply env_locs_monotonic.
+                  unfold FV...
+                + eapply Included_trans; [| eassumption ].
+                  eapply env_locs_monotonic.
+                  unfold FV_cc. now eauto 20 with Ensembles_DB.
+                + eapply Fun_inv_rename_ext.
+                  eapply Fun_inv_Scope_mon. eapply Fun_inv_monotonic.
+                  eauto. simpl in *; omega. now eauto with Ensembles_DB.
+                  symmetry. eapply f_eq_subdomain_antimon; [| eassumption ].
+                  eapply reach'_set_monotonic. eapply env_locs_monotonic...
+              - intros Hc. inv Hc. eauto.
+              - intros Hc.
+                eapply Hd. constructor; eauto. eapply image_monotonic; eauto... }
+          * intros j'.
+            { eapply FV_inv_set_not_in_FVs.
+              - eapply FV_inv_heap_mon; try (now eapply HL.alloc_subheap; eauto).
+                + eapply well_formed_antimon; [| eassumption ].
+                  eapply reach'_set_monotonic. eapply env_locs_monotonic.
+                  unfold FV...
+                + eapply well_formed_antimon; [| eassumption ].
+                  eapply reach'_set_monotonic. eapply env_locs_monotonic.
+                  unfold FV_cc. now eauto 20 with Ensembles_DB.
+                + eapply Included_trans; [| eassumption ].
+                  eapply env_locs_monotonic.
+                  unfold FV...
+                + eapply Included_trans; [| eassumption ].
+                  eapply env_locs_monotonic.
+                  unfold FV_cc. now eauto 20 with Ensembles_DB.
+                + eapply FV_inv_rename_ext.
+                  eapply FV_inv_Scope_mon. eapply FV_inv_monotonic.
+                  eauto. simpl in *; omega. now eauto with Ensembles_DB.
+                  symmetry. eapply f_eq_subdomain_antimon; [| eassumption ].
+                  eapply reach'_set_monotonic. eapply env_locs_monotonic...
+              - intros Hc. inv Hc. eauto.
+              - intros Hc.
+                eapply Hnin. subst; eauto. }
           * assert
               (Hinc :
                  reach' H1'
                         (env_locs (M.set v (Loc l1) rho1)
-                                  (v |: Scope :|: FromList FVs :|: Funs)) \\ [set l1]
+                                  (FV (v |: Scope) Funs FVs)) \\ [set l1]
                         \subset
-                  reach' H1 (env_locs rho1 (Scope :|: FromList FVs :|: Funs))
+                  reach' H1 (env_locs rho1 (FV Scope Funs FVs))
               ).
             { eapply Included_trans. eapply Included_Setminus_compat.
               eapply Included_trans;
                 [| eapply reach'_alloc_set with (H' := H1')
-                                                (S := Scope :|: FromList FVs :|: Funs)];
+                                                (S := FV Scope Funs FVs)];
               try eassumption.
               eapply reach'_set_monotonic. eapply env_locs_monotonic.
               now eauto 20 with Ensembles_DB.
@@ -1289,34 +1639,33 @@ Module ClosureConversionCorrect (H : Heap).
               eapply reach'_set_monotonic. eapply env_locs_monotonic.
               now eauto 20 with Ensembles_DB. }
             eapply injective_subdomain_extend'.
-            { eapply injective_subdomain_antimon. eassumption.
-              eapply Included_trans. eassumption.
-              eapply reach'_set_monotonic. eapply env_locs_monotonic.
-              now eauto 20 with Ensembles_DB. }
+            { eapply injective_subdomain_antimon; eassumption. }
             { intros Hc. eapply image_monotonic in Hc; [| eassumption ].
-              rewrite !env_locs_Union, !reach'_Union, !image_Union in Hc.
-              rewrite cc_approx_env_image_reach in Hc; try eassumption. 
-              rewrite FV_inv_image_reach in Hc; try eassumption.
-              rewrite Fun_inv_image_reach in Hc; try eassumption.
-              rewrite <- !reach'_Union in Hc. eapply reachable_in_dom in Hc.
+              eapply image_FV in Hc; try eassumption.
+              eapply reachable_in_dom in Hc.
               destruct Hc as [vc Hgetc]. erewrite alloc_fresh in Hgetc; eauto. congruence.
               eapply well_formed_antimon; [| eassumption ].
-              rewrite !env_locs_Union, !reach'_Union.
+              unfold FV_cc. rewrite !env_locs_Union, !reach'_Union.
               rewrite <- !Union_assoc. eapply Included_Union_preserv_r.
-              eapply Included_Union_compat. reflexivity. rewrite Union_commut.
-              eapply Included_Union_compat. reflexivity.
+              rewrite !Union_assoc. eapply Included_Union_compat .
+              reflexivity.
               rewrite (reach_unfold H2' (env_locs _ _))...
-              eapply Union_Included. eapply Union_Included.
-              eapply Included_trans; [| eassumption ]. eapply env_locs_monotonic...
+              eapply Union_Included. eapply Included_trans; [| eassumption ].
+              eapply env_locs_monotonic. unfold FV_cc...
               eapply Included_trans; [| eapply reachable_in_dom; eauto ].
               rewrite !env_locs_Union, !reach'_Union.
-              eapply Included_Union_preserv_r. eapply Included_post_reach'.
-              eapply Included_trans; [| eassumption ]. eapply env_locs_monotonic...
+              eapply Included_Union_preserv_r.
+              eapply Included_trans. eapply Included_post_reach'.
+              eapply reach'_set_monotonic. eapply env_locs_monotonic. unfold FV_cc...
               eapply binding_in_map_antimon; [| eassumption ]... }
-          * assert (Hseq : v |: Scope :|: Funs :|: FromList FVs <-->
-                             (Scope :|: Funs :|: FromList FVs) :|: [set v]).
-            { rewrite (Union_commut _ [set v]). rewrite <- !Union_assoc. reflexivity. }
-            rewrite Hseq. eapply well_formed_reach_alloc'; try eassumption.
+          * assert (Hseq : (FV (v |: Scope) Funs FVs) \subset
+                                                      (FV Scope Funs FVs) :|: [set v]).
+            { unfold FV. eapply Union_Included; [| now eauto with Ensembles_DB ].
+              eapply Union_Included; [| now eauto with Ensembles_DB ].
+              eapply Union_Included; [| now eauto with Ensembles_DB ]... }
+            eapply well_formed_antimon. eapply reach'_set_monotonic.
+            eapply env_locs_monotonic. eassumption.
+            eapply well_formed_reach_alloc'; try eassumption.
             rewrite Setminus_Same_set_Empty_set, Union_Empty_set_neut_r.
             eassumption.
             rewrite Setminus_Same_set_Empty_set, Union_Empty_set_neut_r.
@@ -1330,10 +1679,14 @@ Module ClosureConversionCorrect (H : Heap).
             eapply Included_Union_compat. reflexivity.
             eapply Included_trans; [| eassumption ].
             eapply env_locs_monotonic. now eauto 20 with Ensembles_DB.
-          * assert (Hseq : v |: Scope :|: image σ Funs :|: [set Γ] <-->
-                             (Scope :|: image σ Funs :|: [set Γ]) :|: [set v]).
-            { rewrite (Union_commut _ [set v]). rewrite <- !Union_assoc. reflexivity. }
-            rewrite Hseq. eapply well_formed_reach_alloc; eauto.
+          * assert (Hseq : (FV_cc (v |: Scope) Funs σ Γ) \subset
+                                                      (FV_cc Scope Funs σ Γ) :|: [set v]).
+            { unfold FV_cc. eapply Union_Included; [| now eauto with Ensembles_DB ].
+              eapply Union_Included; [| now eauto 20 with Ensembles_DB ].
+              eapply Union_Included; [| now eauto with Ensembles_DB ]... }
+            eapply well_formed_antimon. eapply reach'_set_monotonic.
+            eapply env_locs_monotonic. eassumption.
+            eapply well_formed_reach_alloc; eauto.
             eapply well_formed_antimon; [| eassumption ].
             eapply reach'_set_monotonic. eapply env_locs_monotonic...
             eapply Included_trans;[| eassumption ].
