theories/L6_PCPS/Heap/compat.v
@@ -6,7 +6,7 @@
 From Coq Require Import NArith.BinNat Relations.Relations MSets.MSets
                         MSets.MSetRBT Lists.List omega.Omega Sets.Ensembles.
 From L6 Require Import functions cps ctx eval cps_util identifiers ctx Ensembles_util
-     List_util Heap.heap Heap.heap_defs Heap.space_sem
+     List_util Heap.heap Heap.heap_defs Heap.space_sem Heap.closure_conversion
      Heap.cc_log_rel tactics.
 From compcert Require Import lib.Coqlib.
 
